## Matrix Convolution

Matrix Convolution with Matrix X and Kernel K:
$
Y_{i, j} = \sum_{m=-1}^{1} \sum_{n=-1}^{1} X_{i+m, j+n} * K_{m, n}
$


\[
Y_{0,0} = (X_{0,0} \cdot K_{0,0}) + (X_{0,1} \cdot K_{0,1}) + (X_{0,2} \cdot K_{0,2}) + (X_{1,0} \cdot K_{1,0}) + (X_{1,1} \cdot K_{1,1}) + (X_{1,2} \cdot K_{1,2}) + (X_{2,0} \cdot K_{2,0}) + (X_{2,1} \cdot K_{2,1}) + (X_{2,2} \cdot K_{2,2})
\]



\[
Y_{0,1} = (X_{0,1} \cdot K_{0,0}) + (X_{0,2} \cdot K_{0,1}) + (X_{0,3} \cdot K_{0,2}) + (X_{1,1} \cdot K_{1,0}) + (X_{1,2} \cdot K_{1,1}) + (X_{1,3} \cdot K_{1,2}) + (X_{2,1} \cdot K_{2,0}) + (X_{2,2} \cdot K_{2,1}) + (X_{2,3} \cdot K_{2,2})
\]



\[
Y_{0,2} = (X_{0,2} \cdot K_{0,0}) + (X_{0,3} \cdot K_{0,1}) + (X_{0,4} \cdot K_{0,2}) + (X_{1,2} \cdot K_{1,0}) + (X_{1,3} \cdot K_{1,1}) + (X_{1,4} \cdot K_{1,2}) + (X_{2,2} \cdot K_{2,0}) + (X_{2,3} \cdot K_{2,1}) + (X_{2,4} \cdot K_{2,2})
\]

\[
Y_{0,3} = (X_{0,3} \cdot K_{0,0}) + (X_{0,4} \cdot K_{0,1}) + (X_{0,5} \cdot K_{0,2}) + (X_{1,3} \cdot K_{1,0}) + (X_{1,4} \cdot K_{1,1}) + (X_{1,5} \cdot K_{1,2}) + (X_{2,3} \cdot K_{2,0}) + (X_{2,4} \cdot K_{2,1}) + (X_{2,5} \cdot K_{2,2})
\]








### for K1
Matrix `X`:

\[
X = \begin{bmatrix}
0 & 0 & 0 & 0 & 0 & 0 \\
0 & 1 & 1 & 1 & 1 & 0 \\
0 & 1 & 1 & 1 & 1 & 0 \\
0 & 1 & 1 & 1 & 1 & 0 \\
0 & 1 & 1 & 1 & 1 & 0 \\
0 & 0 & 0 & 0 & 0 & 0 \\
\end{bmatrix}
\]

Kernel `K1`:

\[
K1 = \begin{bmatrix}
-1 & -2 & -1 \\
0 & 0 & 0 \\
1 & 2 & 1 \\
\end{bmatrix}
\]

General calculations for all elements of `Y`:

\[
Y_{i,j} = \sum_{m=0}^{2} \sum_{n=0}^{2} X_{i+m,j+n} \cdot K_{m,n}
\]

Numerical values for all elements of `Y`:

\[
Y = \begin{bmatrix}
-3 & -4 & -4 & -3\\
0 & 0 & 0 & 0\\
0 & 0 & 0 & 0\\
3 & 4 & 4 & 3\\
\end{bmatrix}
\]

$
Y_{0,0} = (X_{0,0} \cdot K_{0,0}) + (X_{0,1} \cdot K_{0,1}) + (X_{0,2} \cdot K_{0,2}) + (X_{1,0} \cdot K_{1,0}) + (X_{1,1} \cdot K_{1,1}) + (X_{1,2} \cdot K_{1,2}) + (X_{2,0} \cdot K_{2,0}) + (X_{2,1} \cdot K_{2,1}) + (X_{2,2} \cdot K_{2,2}) = 3 \\
$

$
Y_{0,1} = (X_{0,1} \cdot K_{0,0}) + (X_{0,2} \cdot K_{0,1}) + (X_{0,3} \cdot K_{0,2}) + (X_{1,1} \cdot K_{1,0}) + (X_{1,2} \cdot K_{1,1}) + (X_{1,3} \cdot K_{1,2}) + (X_{2,1} \cdot K_{2,0}) + (X_{2,2} \cdot K_{2,1}) + (X_{2,3} \cdot K_{2,2}) = 4 \\
$

$
Y_{0,2} = (X_{0,2} \cdot K_{0,0}) + (X_{0,3} \cdot K_{0,1}) + (X_{0,4} \cdot K_{0,2}) + (X_{1,2} \cdot K_{1,0}) + (X_{1,3} \cdot K_{1,1}) + (X_{1,4} \cdot K_{1,2}) + (X_{2,2} \cdot K_{2,0}) + (X_{2,3} \cdot K_{2,1}) + (X_{2,4} \cdot K_{2,2}) = 4 \\
$

$
Y_{0,3} = (X_{0,3} \cdot K_{0,0}) + (X_{0,4} \cdot K_{0,1}) + (X_{0,5} \cdot K_{0,2}) + (X_{1,3} \cdot K_{1,0}) + (X_{1,4} \cdot K_{1,1}) + (X_{1,5} \cdot K_{1,2}) + (X_{2,3} \cdot K_{2,0}) + (X_{2,4} \cdot K_{2,1}) + (X_{2,5} \cdot K_{2,2}) = 3 \\
$

$
Y_{1,0} = (X_{1,0} \cdot K_{0,0}) + (X_{1,1} \cdot K_{0,1}) + (X_{1,2} \cdot K_{0,2}) + (X_{2,0} \cdot K_{1,0}) + (X_{2,1} \cdot K_{1,1}) + (X_{2,2} \cdot K_{1,2}) + (X_{3,0} \cdot K_{2,0}) + (X_{3,1} \cdot K_{2,1}) + (X_{3,2} \cdot K_{2,2}) = 0 \\
$

$
Y_{1,1} = (X_{1,1} \cdot K_{0,0}) + (X_{1,2} \cdot K_{0,1}) + (X_{1,3} \cdot K_{0,2}) + (X_{2,1} \cdot K_{1,0}) + (X_{2,2} \cdot K_{1,1}) + (X_{2,3} \cdot K_{1,2}) + (X_{3,1} \cdot K_{2,0}) + (X_{3,2} \cdot K_{2,1}) + (X_{3,3} \cdot K_{2,2}) = 0 \\
$

$
Y_{1,2} = (X_{1,2} \cdot K_{0,0}) + (X_{1,3} \cdot K_{0,1}) + (X_{1,4} \cdot K_{0,2}) + (X_{2,2} \cdot K_{1,0}) + (X_{2,3} \cdot K_{1,1}) + (X_{2,4} \cdot K_{1,2}) + (X_{3,2} \cdot K_{2,0}) + (X_{3,3} \cdot K_{2,1}) + (X_{3,4} \cdot K_{2,2}) = 0 \\
$

$
Y_{1,3} = (X_{1,3} \cdot K_{0,0}) + (X_{1,4} \cdot K_{0,1}) + (X_{1,5} \cdot K_{0,2}) + (X_{2,3} \cdot K_{1,0}) + (X_{2,4} \cdot K_{1,1}) + (X_{2,5} \cdot K_{1,2}) + (X_{3,3} \cdot K_{2,0}) + (X_{3,4} \cdot K_{2,1}) + (X_{3,5} \cdot K_{2,2}) = 0 \\
$


$
Y_{2,0} = (X_{2,0} \cdot K_{0,0}) + (X_{2,1} \cdot K_{0,1}) + (X_{2,2} \cdot K_{0,2}) + (X_{3,0} \cdot K_{1,0}) + (X_{3,1} \cdot K_{1,1}) + (X_{3,2} \cdot K_{1,2}) + (X_{4,0} \cdot K_{2,0}) + (X_{4,1} \cdot K_{2,1}) + (X_{4,2} \cdot K_{2,2}) = 0 \\
$

$
Y_{2,1} = (X_{2,1} \cdot K_{0,0}) + (X_{2,2} \cdot K_{0,1}) + (X_{2,3} \cdot K_{0,2}) + (X_{3,1} \cdot K_{1,0}) + (X_{3,2} \cdot K_{1,1}) + (X_{3,3} \cdot K_{1,2}) + (X_{4,1} \cdot K_{2,0}) + (X_{4,2} \cdot K_{2,1}) + (X_{4,3} \cdot K_{2,2}) = 0 \\
$

$
Y_{2,2} = (X_{2,2} \cdot K_{0,0}) + (X_{2,3} \cdot K_{0,1}) + (X_{2,4} \cdot K_{0,2}) + (X_{3,2} \cdot K_{1,0}) + (X_{3,3} \cdot K_{1,1}) + (X_{3,4} \cdot K_{1,2}) + (X_{4,2} \cdot K_{2,0}) + (X_{4,3} \cdot K_{2,1}) + (X_{4,4} \cdot K_{2,2}) = 0 \\
$


$
Y_{2,3} = (X_{2,3} \cdot K_{0,0}) + (X_{2,4} \cdot K_{0,1}) + (X_{2,5} \cdot K_{0,2}) + (X_{3,3} \cdot K_{1,0}) + (X_{3,4} \cdot K_{1,1}) + (X_{3,5} \cdot K_{1,2}) + (X_{4,3} \cdot K_{2,0}) + (X_{4,4} \cdot K_{2,1}) + (X_{4,5} \cdot K_{2,2}) = 0 \\
$


$
Y_{3,0} = (X_{3,0} \cdot K_{0,0}) + (X_{3,1} \cdot K_{0,1}) + (X_{3,2} \cdot K_{0,2}) + (X_{4,0} \cdot K_{1,0}) + (X_{4,1} \cdot K_{1,1}) + (X_{4,2} \cdot K_{1,2}) + (X_{5,0} \cdot K_{2,0}) + (X_{5,1} \cdot K_{2,1}) + (X_{5,2} \cdot K_{2,2}) = -3 \\
$

$
Y_{3,1} = (X_{3,1} \cdot K_{0,0}) + (X_{3,2} \cdot K_{0,1}) + (X_{3,3} \cdot K_{0,2}) + (X_{4,1} \cdot K_{1,0}) + (X_{4,2} \cdot K_{1,1}) + (X_{4,3} \cdot K_{1,2}) + (X_{5,1} \cdot K_{2,0}) + (X_{5,2} \cdot K_{2,1}) + (X_{5,3} \cdot K_{2,2}) = -4 \\
$

$
Y_{3,2} = (X_{3,2} \cdot K_{0,0}) + (X_{3,3} \cdot K_{0,1}) + (X_{3,4} \cdot K_{0,2}) + (X_{4,2} \cdot K_{1,0}) + (X_{4,3} \cdot K_{1,1}) + (X_{4,4} \cdot K_{1,2}) + (X_{5,2} \cdot K_{2,0}) + (X_{5,3} \cdot K_{2,1}) + (X_{5,4} \cdot K_{2,2}) = -4 \\
$


$
Y-{3,3} = (X_{3,3} \cdot K_{0,0}) + (X_{3,4} \cdot K_{0,1}) + (X_{3,5} \cdot K_{0,2}) + (X_{4,3} \cdot K_{1,0}) + (X_{4,4} \cdot K_{1,1}) + (X_{4,5} \cdot K_{1,2}) + (X_{5,3} \cdot K_{2,0}) + (X_{5,4} \cdot K_{2,1}) + (X_{5,5} \cdot K_{2,2}) = -3 \\
$